Update the ssr examples

examples/ssr/Context.v
@@ -1,25 +1,29 @@
 (** * Context
 
     Support for dependent contexts with the right reduction behaviour. *)
-Require Import mathcomp.ssreflect.ssreflect.
-From mathcomp Require Import ssreflect ssrfun ssrbool eqtype ssrnat seq.
+From Coq Require Import ssreflect ssrfun ssrbool Lists.List.
 Require Import AutosubstSsr.
 
-Definition get {T} `{Ids T} (Gamma : seq T) (n : var) : T :=
-  nth (ids 0) Gamma n.
+Definition get {T} `{!Ids T} (Gamma : list T) (n : var) : T :=
+  nth n Gamma (ids 0).
 Arguments get {T _} Gamma n.
 
-Fixpoint dget {T} `{Ids T} `{Subst T} (Gamma : list T) (n : var) {struct n} : T :=
+Fixpoint dget {T} `{!Ids T, !Subst T} (Gamma : list T) (n : var) {struct n} : T :=
   match Gamma, n with
-    | [::], _ => ids 0
+    | nil, _ => ids 0
     | A :: _, 0 => A.[ren (+1)]
-    | _ :: Gamma, n.+1 => (dget Gamma n).[ren (+1)]
+    | _ :: Gamma, (S n) => (dget Gamma n).[ren (+1)]
   end.
 Arguments dget {T _ _} Gamma n.
 
 Lemma get_map {T} `{Ids T} (f : T -> T) Gamma n :
-  n < size Gamma -> get (map f Gamma) n = f (get Gamma n).
-Proof. exact: nth_map. Qed.
+  n < length Gamma -> get (map f Gamma) n = f (get Gamma n).
+Proof.
+  rewrite -(map_length f).
+  intros Hn. rewrite /get. etransitivity.
+  2:{ apply map_nth. }
+  by apply nth_indep.
+Qed.
 
 (* Local Variables: *)
 (* coq-load-path: (("." "Ssr")) *)
