examples/ssr/BetaSubstitution.v
@@ -1,7 +1,8 @@
 (** * Correctness of Single Variable Substitutions *)
-Require Import mathcomp.ssreflect.ssreflect.
-From mathcomp Require Import ssreflect ssrfun ssrbool eqtype ssrnat seq.
+From Coq Require Import ssreflect ssrfun ssrbool.
+From Coq Require Import Arith.
 Require Import Autosubst.
+Require Import Lia.
 
 Set Implicit Arguments.
 Unset Strict Implicit.
@@ -22,17 +23,17 @@ Instance SubstLemmas_term : SubstLemmas term. derive. Qed.
 
 Fixpoint lift_at (d k : nat) (s : term) : term :=
   match s with
-    | Var i   => if i < d then Var i else Var (k + i)
+    | Var i   => if i <? d then Var i else Var (k + i)
     | App s t => App (lift_at d k s) (lift_at d k t)
-    | Lam s   => Lam (lift_at d.+1 k s)
+    | Lam s   => Lam (lift_at (S d) k s)
   end.
 Notation lift := (lift_at 0).
 
 Fixpoint sbst_at (d : nat) (t s : term) : term :=
   match s with
-    | Var x => if x < d then Var x else if x == d then lift d t else Var x.-1
+    | Var x => if x <? d then Var x else if x =? d then lift d t else Var (x-1)
     | App s1 s2 => App (sbst_at d t s1) (sbst_at d t s2)
-    | Lam s => Lam (sbst_at d.+1 t s)
+    | Lam s => Lam (sbst_at (S d) t s)
   end.
 Notation sbst := (sbst_at 0).
 
@@ -56,11 +57,11 @@ Qed.
 
 Lemma upnP n sigma x :
   upn n sigma x =
-    if x < n then Var x else (sigma (x - n)).[ren (+n)].
+    if x <? n then Var x else (sigma (x - n)).[ren (+n)].
 Proof.
   case: ifPn.
   - elim: x n =>[|x ih][|n]//=/ih e. rewrite iterate_S. asimpl. by rewrite e.
-  - rewrite -leqNgt. elim: x n => [|x ih][|n]; try autosubst. by case: n.
+  - rewrite -Nat.leb_antisym. elim: x n => [|x ih][|n]; try autosubst. by case: n.
     move=>/ih e. rewrite iterate_S. asimpl. rewrite e. autosubst.
 Qed.
 
@@ -68,11 +69,14 @@ Lemma sbst_at_sound d t s :
   sbst_at d t s = s.[upn d (t .: ids)].
 Proof.
   elim: s d => /=[x|s1 ih1 s2 ih2|s ih] d.
-  - rewrite lift_sound. rewrite upnP. case: ifPn => //=. rewrite -leqNgt => le.
-    case: ifP => [/eqP->|/eqP/eqP]. by rewrite subnn. rewrite neq_ltn =>/orP[|{le}]//.
-    move=> /leq_trans/(_ le). by rewrite ltnn. rewrite -subn_gt0 => p.
-    move: (p) => /ltn_predK<-/=. rewrite/ids/Ids_term. f_equal.
-    case: x p => //= n p. rewrite subSKn plusE subnKC //. by rewrite subn_gt0 in p.
+  - rewrite lift_sound. rewrite upnP. case: ifPn => //=.
+    rewrite -Nat.leb_antisym => /(elimT (Nat.leb_spec0 _ _)) le.
+    case: ifP => [/(elimT (Nat.eqb_spec _ _)) ->|].
+    { by rewrite Nat.sub_diag. }
+    move /(elimF (Nat.eqb_spec _ _)) /not_eq =>[?|lt]; first lia.
+    assert (x - d > 0) by lia.
+    assert (x - d = S ((x - d) - 1)) as -> by lia.
+    asimpl. rewrite /ids /Ids_term. f_equal. lia.
   - by rewrite ih1 ih2.
   - by rewrite ih.
 Qed.
